Kraken/X64/Sep.lean
@@ -27,3 +27,52 @@ theorem load_sep (s : MachineData) (addr : BitVec 64) (w : Width) (ret : w.type 
       require_read_access addr w (fun _ => ret (.ofInt w.bits (Int.ofBytes bs)) s) := by
   simp only [MachineData.load,
     Mem.loadInt_sep bs addr w.bytes R s.dmem h_mem h_len (by cases w <;> decide)]
+
+@[kspec]
+theorem loadAvx_sep (s : MachineData) (addr : BitVec 64) (w : AvxWidth) (ret : w.type → MachineData → Effects)
+    (bs : List UInt8) (R : DataMem → Prop)
+    (h_mem : s.dmem =⋆ Eq (bs.At addr) ⋆ R)
+    (h_len : bs.length = w.bytes) :
+    MachineData.loadAvx s addr w ret false =
+      require_read_access addr .W64 (fun _ => ret (.ofInt w.bits (Int.ofBytes bs)) s) := by
+  simp only [MachineData.loadAvx, isAligned]
+  simp only [Mem.loadInt_sep bs addr w.bytes R s.dmem h_mem h_len (by cases w <;> decide)]
+  -- Use reflexivity to evaluate the definitional equality and close the goal!
+  rfl
+
+@[kspec]
+theorem storeAvx_sep (s : MachineData) (addr : BitVec 64) (w : AvxWidth) (v : w.type) (ret : MachineData → Effects)
+    (bs : List UInt8) (R : DataMem → Prop)
+    (h_mem : s.dmem =⋆ Eq (bs.At addr) ⋆ R)
+    (h_len : bs.length = w.bytes) :
+    MachineData.storeAvx s addr v ret false =
+      require_write_access addr .W64 (fun _ =>
+        ret { s with dmem := Mem.storeInt s.dmem addr w.bytes v.toInt }) := by
+  simp only [MachineData.storeAvx, isAligned]
+  simp only [Mem.loadInt_sep bs addr w.bytes R s.dmem h_mem h_len (by cases w <;> decide)]
+  rfl
+
+@[kspec]
+theorem loadAvx_sep_aligned (s : MachineData) (addr : BitVec 64) (w : AvxWidth) (ret : w.type → MachineData → Effects)
+    (bs : List UInt8) (R : DataMem → Prop)
+    (h_mem : s.dmem =⋆ Eq (bs.At addr) ⋆ R)
+    (h_len : bs.length = w.bytes)
+    (h_align : isAligned w.bytes addr = true) :
+    MachineData.loadAvx s addr w ret true =
+      require_read_access addr .W64 (fun _ => ret (.ofInt w.bits (Int.ofBytes bs)) s) := by
+  simp only [MachineData.loadAvx, h_align, Bool.and_false, if_false]
+  simp only [Mem.loadInt_sep bs addr w.bytes R s.dmem h_mem h_len (by cases w <;> decide)]
+  rfl
+
+@[kspec]
+theorem storeAvx_sep_aligned (s : MachineData) (addr : BitVec 64) (w : AvxWidth) (v : w.type) (ret : MachineData → Effects)
+    (bs : List UInt8) (R : DataMem → Prop)
+    (h_mem : s.dmem =⋆ Eq (bs.At addr) ⋆ R)
+    (h_len : bs.length = w.bytes)
+    (h_align : isAligned w.bytes addr = true) :
+    MachineData.storeAvx s addr v ret true =
+      require_write_access addr .W64 (fun _ =>
+        ret { s with dmem := Mem.storeInt s.dmem addr w.bytes v.toInt }) := by
+  simp only [MachineData.storeAvx, h_align, Bool.and_false, if_false]
+  simp only [Mem.loadInt_sep bs addr w.bytes R s.dmem h_mem h_len (by cases w <;> decide)]
+  rfl
